\documentclass{article}
\usepackage{graphicx} % Required for inserting images
\usepackage{amsmath}
\usepackage{amssymb}
\usepackage{amsthm}

\theoremstyle{definition}
\newtheorem{thm}{Theorem}[section]
\theoremstyle{definition}
\newtheorem{defn}[thm]{Definition}
\theoremstyle{definition}
\newtheorem{ex}[thm]{Example}
\newtheorem{prop}[thm]{Proposition}
\newtheorem{corr}[thm]{Corollary}


\title{sizes of numerical sets}
\date{Summer 2024}
\begin{document}
\maketitle

\begin{prop}
    Let $T$ be a numerical set. Suppose $A(T) = S$. Then 
    $$|\lambda(T)| = |\lambda(S)| + |A| - |B|,$$

    where $A, B$ are defined as follows: 
    $$A = \{(n, h)\mid n\in I, h\notin T, n <h\}$$
    $$ B = \{(n, h)\mid n \in S, h\in I, n <h \}.$$

    \textit{Proof.} We recall the following:
    $$|\lambda(S)| = \#\{(n, h) \mid n \in S, h\notin S, n<h\}$$
    $$|\lambda(T)| = \#\{(n, h)\mid n \in T, h\notin T, n<h\}.$$
    Since $T= S\cup I$ for some order ideal $I$ with $S \cap I = \varnothing$, we have that 
    $$|\lambda(T)| = \#\{(n,h)\mid n\in S, h\notin T, n<h\} + \#\{(n,h)\mid n\in I, h\notin T, n<h\},$$
that is, 
    $$|\lambda(T)| = \#\{(n,h)\mid n\in S, h\notin T, n<h\} + |A|.$$
We further note that $h \notin T$ if and only if $h\notin S$ and $h\notin I$, and realize that
    
    $$|\lambda(T)| = \#\{(n,h)\mid n\in S, h\notin S, n<h\} - \#\{(n, h)\mid n\in S, h\in I, n<h\} + |A|.$$
Lastly, we recall the definitions above, and obtain 
    $$|\lambda(T)| = |\lambda(S)| + |A| - |B|,$$
    as desired. $\blacksquare$
    
\end{prop}

\begin{corr}
    $|\lambda(T)| < |\lambda(S)|$ if and only if $|A| < |B|.$
\end{corr}

\begin{corr}
    Let $T$ be a numerical set. Suppose $A(T) = S$. Then 
    $$|\lambda(T)| = |\lambda(S)| + \#\{(n, h)\mid n\in I, h\notin S, n <h\} - \#\{(n, h)\mid n \in T, h\in I, n <h \}.$$

    \textit{Proof.} We only need to note that 
    $$|A| = \#\{(n, h) \mid n \in I, h \notin S, n<h\} - \#\{(n, h) \mid n\in T, h \in T, n< h\}.$$
    Rearranging thereafter leads to the stated equality. $\blacksquare$
\end{corr}

\begin{corr}
    $|\lambda(T)|=|\lambda(S)| + g(S)\cdot|I|-\frac{1}{2}|I|\cdot(|I|-1) - \sum I_j$
\end{corr}


\end{document}